reprove push, pop

theories/resizing/code.v
@@ -223,10 +223,10 @@ End code.
 (** Ghost state for the deque *)
 
 Class dequeG Σ := DequeG {
-    (* invariant *)
+    (* spec *)
     deque_tokG :> inG Σ (excl_authR $ listO valO);
-    deque_popG :> ghost_varG Σ bool;
-    eraG :> ghost_varG Σ (nat * list val);
+    (* info: era, arrptr, arr, bot, popping *)
+    deque_infoG :> ghost_varG Σ (nat * loc * list val * nat * bool);
     (* RA *)
     topbotG :> mono_natG Σ;
     topeltG :> mono_listG val Σ;
@@ -237,8 +237,7 @@ Class dequeG Σ := DequeG {
 Definition dequeΣ : gFunctors :=
   #[ (*invariant *)
     GFunctor (excl_authR $ listO valO);
-    ghost_varΣ bool;
-    ghost_varΣ (nat * list val);
+    ghost_varΣ (nat * loc * list val * nat * bool);
     (* RA *)
     mono_natΣ;
     mono_listΣ val;
@@ -252,14 +251,14 @@ Proof. solve_inG. Qed.
 Section dqst.
   Context `{!heapGS Σ, !dequeG Σ}.
   Notation iProp := (iProp Σ).
-  Definition glob_gnames : Type := gname*gname*gname*gname.
+  Definition dqst_gnames : Type := gname*gname*gname*gname.
 
   Definition top_bot_state (t b : nat) : nat :=
     2*t + (if bool_decide (t < b) then 1 else 0).
 
-  Definition dqst_frag (γglob : glob_gnames) (era : nat)
+  Definition dqst_frag (γdqst : dqst_gnames) (era : nat)
   (arr : loc) (l : list val) (t b : nat) : iProp :=
-    let (γ'              , γmus) := γglob in
+    let (γ'              , γmus) := γdqst in
     let (γ''      , γroom) := γ' in
     let (γtb, γelt) := γ'' in
     ∃ (γtbe : gname),
@@ -279,9 +278,9 @@ Section dqst.
       mono_list_lb_own γroom room
     ).
 
-  Definition dqst_archived (γglob : glob_gnames) (era : nat)
+  Definition dqst_archived (γdqst : dqst_gnames) (era : nat)
   (arr : loc) (l : list val) (t b : nat) : iProp :=
-    let (γ'              , γmus) := γglob in
+    let (γ'              , γmus) := γdqst in
     let (γ''      , γroom) := γ' in
     let (γtb, γelt) := γ'' in
     ∃ (γtbe : gname),
@@ -306,9 +305,9 @@ Section dqst.
     (* persistent circle *)
     arr ↦∗□ l.
 
-  Definition dqst_auth (γglob : glob_gnames) (era : nat)
+  Definition dqst_auth (γdqst : dqst_gnames) (era : nat)
   (arr : loc) (l : list val) (t b : nat) : iProp :=
-    let (γ'              , γmus) := γglob in
+    let (γ'              , γmus) := γdqst in
     let (γ''      , γroom) := γ' in
     let (γtb, γelt) := γ'' in
     ∃ (γtbe : gname),
@@ -331,7 +330,7 @@ Section dqst.
       mono_list_auth_own γroom 1 (proom ++ [(γtbe, arr, length l)]) ∗
       mono_list_auth_own γmus 1 museum ∗
       [∗ list] i ↦ gcl ; ltbi ∈ proom ; museum, (
-        dqst_archived γglob i (gcl.1.2) (ltbi.1.1) (ltbi.1.2) (ltbi.2)
+        dqst_archived γdqst i (gcl.1.2) (ltbi.1.1) (ltbi.1.2) (ltbi.2)
       )
     ).
 
@@ -339,25 +338,25 @@ Section dqst.
   Ltac desγ H :=
     destruct H as (((γtb, γelt), γroom), γmuseum).
 
-  Global Instance dqst_frag_timeless γglob era ca l t b :
-    Timeless (dqst_frag γglob era ca l t b).
-  Proof. desγ γglob. apply _. Qed.
+  Global Instance dqst_frag_timeless γdqst era ca l t b :
+    Timeless (dqst_frag γdqst era ca l t b).
+  Proof. desγ γdqst. apply _. Qed.
 
-  Global Instance dqst_frag_persistent γglob era ca l t b :
-    Persistent (dqst_frag γglob era ca l t b).
-  Proof. desγ γglob. apply _. Qed.
+  Global Instance dqst_frag_persistent γdqst era ca l t b :
+    Persistent (dqst_frag γdqst era ca l t b).
+  Proof. desγ γdqst. apply _. Qed.
   
-  Global Instance dqst_archived_timeless γglob era ca l t b :
-    Timeless (dqst_archived γglob era ca l t b).
-  Proof. desγ γglob. apply _. Qed.
+  Global Instance dqst_archived_timeless γdqst era ca l t b :
+    Timeless (dqst_archived γdqst era ca l t b).
+  Proof. desγ γdqst. apply _. Qed.
 
-  Global Instance dqst_archived_persistent γglob era ca l t b :
-    Persistent (dqst_archived γglob era ca l t b).
-  Proof. desγ γglob. apply _. Qed.
+  Global Instance dqst_archived_persistent γdqst era ca l t b :
+    Persistent (dqst_archived γdqst era ca l t b).
+  Proof. desγ γdqst. apply _. Qed.
 
-  Global Instance dqst_auth_timeless γglob era ca l t b :
-    Timeless (dqst_auth γglob era ca l t b).
-  Proof. desγ γglob. apply _. Qed.
+  Global Instance dqst_auth_timeless γdqst era ca l t b :
+    Timeless (dqst_auth γdqst era ca l t b).
+  Proof. desγ γdqst. apply _. Qed.
   
   Lemma top_bot_state_le t1 b1 t2 b2 :
     top_bot_state t1 b1 ≤ top_bot_state t2 b2 ↔
@@ -366,8 +365,8 @@ Section dqst.
 
   Lemma dqst_auth_alloc ca l :
     length l ≠ 0 →
-    ⊢ |==> ∃ (γglob : glob_gnames),
-      dqst_auth γglob 0 ca l 1 1.
+    ⊢ |==> ∃ (γdqst : dqst_gnames),
+      dqst_auth γdqst 0 ca l 1 1.
   Proof.
     intros Hl. unfold dqst_auth.
     iMod (mono_nat_own_alloc 2) as (γtb) "[tb _]".
@@ -380,12 +379,12 @@ Section dqst.
     iSplitL "topelt"; fr. fr.
   Qed.
 
-  Lemma dqst_frag_agree γglob era ca1 l1 t1 b1 ca2 l2 t2 b2 :
-    dqst_frag γglob era ca1 l1 t1 b1 -∗
-    dqst_frag γglob era ca2 l2 t2 b2 -∗
+  Lemma dqst_frag_agree γdqst era ca1 l1 t1 b1 ca2 l2 t2 b2 :
+    dqst_frag γdqst era ca1 l1 t1 b1 -∗
+    dqst_frag γdqst era ca2 l2 t2 b2 -∗
     ⌜ca1 = ca2 ∧ length l1 = length l2⌝.
   Proof.
-    desγ γglob.
+    desγ γdqst.
     iIntros "F1 F2".
       iDestruct "F1" as (γtbe1) "(%Hlt1 & tb1 & elt1 & muse1)".
       iDestruct "muse1" as (room1) "[%Hroom1 Lb1]".
@@ -398,11 +397,11 @@ Section dqst.
       rewrite Hroom2 in Hroom1. by injection Hroom1.
   Qed.
 
-  Lemma dqst_get_frag γglob era ca l t b :
-    dqst_auth γglob era ca l t b -∗
-    dqst_frag γglob era ca l t b.
+  Lemma dqst_get_frag γdqst era ca l t b :
+    dqst_auth γdqst era ca l t b -∗
+    dqst_frag γdqst era ca l t b.
   Proof with extended_auto.
-    desγ γglob.
+    desγ γdqst.
     iIntros "Auth".
       iDestruct "Auth" as (γtbeO) "(%HltO & [tbO tbeO] & eltO & museO)".
       iDestruct "eltO" as (elts) "[Elt %Heltslen]".
@@ -418,15 +417,15 @@ Section dqst.
     - fr. rewrite lookup_app_r... replace (era - length room) with 0...
   Qed.
 
-  Lemma dqst_get_archived γglob era1 ca1 l1 t1 b1
+  Lemma dqst_get_archived γdqst era1 ca1 l1 t1 b1
   era2 ca2 l2 t2 b2 :
     (* era1 is later than era2 *)
     era1 ≠ era2 →
-    dqst_auth γglob era1 ca1 l1 t1 b1 -∗
-    dqst_frag γglob era2 ca2 l2 t2 b2 -∗
-    ∃ l' t' b', dqst_archived γglob era2 ca2 l' t' b'.
+    dqst_auth γdqst era1 ca1 l1 t1 b1 -∗
+    dqst_frag γdqst era2 ca2 l2 t2 b2 -∗
+    ∃ l' t' b', dqst_archived γdqst era2 ca2 l' t' b'.
   Proof with extended_auto.
-    desγ γglob.
+    desγ γdqst.
     iIntros (Hneq) "Auth F".
       iDestruct "Auth" as (γtbeO) "(%HltO & tbO & eltO & museO)".
       iDestruct "museO" as (room museum) "museO".
@@ -446,17 +445,17 @@ Section dqst.
     iDestruct (big_sepL2_lookup with "Archives") as "Arch2"...
   Qed.
 
-  Lemma dqst_get_lb γglob era1 ca1 l1 t1 b1
+  Lemma dqst_get_lb γdqst era1 ca1 l1 t1 b1
   era2 ca2 l2 t2 b2 :
     (* era1 is later than era2 *)
-    dqst_auth γglob era1 ca1 l1 t1 b1 -∗
-    dqst_frag γglob era2 ca2 l2 t2 b2 -∗
+    dqst_auth γdqst era1 ca1 l1 t1 b1 -∗
+    dqst_frag γdqst era2 ca2 l2 t2 b2 -∗
     ⌜t2 ≤ t1 ∧ (
       (t2 = t1 ∧ t2 < b2) →
       (t1 < b1 ∧ mod_get l2 t2 = mod_get l1 t1)
     )⌝.
   Proof with extended_auto.
-    desγ γglob.
+    desγ γdqst.
     iIntros "Auth F".
       iDestruct "Auth" as (γtbeO) "(%HltO & [tbO tbeO] & eltO & museO)".
       iDestruct "F" as (γtbe) "(%Hlt & [tb tbe] & elt & muse)".
@@ -473,35 +472,35 @@ Section dqst.
     rewrite Hget Helts...
   Qed.
 
-  Lemma dqst_archived_get_array γglob era ca l t b :
-    dqst_archived γglob era ca l t b -∗
+  Lemma dqst_archived_get_array γdqst era ca l t b :
+    dqst_archived γdqst era ca l t b -∗
     ca ↦∗□ l.
   Proof.
-    desγ γglob.
+    desγ γdqst.
     iIntros "Arc".
     by iDestruct "Arc" as (γtbeA) "(_&_&_&_& pers)".
   Qed.
 
-  Lemma dqst_archived_get_frag γglob era ca l t b :
-    dqst_archived γglob era ca l t b -∗
-    dqst_frag γglob era ca l t b.
+  Lemma dqst_archived_get_frag γdqst era ca l t b :
+    dqst_archived γdqst era ca l t b -∗
+    dqst_frag γdqst era ca l t b.
   Proof.
-    desγ γglob.
+    desγ γdqst.
     iIntros "Arc".
       iDestruct "Arc" as (γtbeA) "(%Hlt & [tb tbe] & elt & muse & pers)".
       iDestruct "muse" as (room museum) "(%Hroom & Hmuseum & Room & Museum)".
     fr. fr. by iApply mono_nat_persistent_lb_own_get.
   Qed.
 
-  Lemma dqst_archived_get_lb γglob era ca l1 t1 b1 l2 t2 b2 :
-    dqst_archived γglob era ca l1 t1 b1 -∗
-    dqst_frag γglob era ca l2 t2 b2 -∗
+  Lemma dqst_archived_get_lb γdqst era ca l1 t1 b1 l2 t2 b2 :
+    dqst_archived γdqst era ca l1 t1 b1 -∗
+    dqst_frag γdqst era ca l2 t2 b2 -∗
     ⌜t2 ≤ t1 ∧ (
       (t2 = t1 ∧ t2 < b2) →
       (t1 < b1 ∧ mod_get l2 t2 = mod_get l1 t1)
     )⌝.
   Proof with extended_auto.
-    desγ γglob.
+    desγ γdqst.
     iIntros "Arc F".
       iDestruct "Arc" as (γtbeA) "(%Hlt1 & [tb1 tbe1] & elt1 & muse1 & pers1)".
       iDestruct "muse1" as (room1 museum1) "muse1".
@@ -525,11 +524,11 @@ Section dqst.
     - rewrite -lookup_lt_is_Some -Hget1. apply mod_get_is_Some...
   Qed.
 
-  Lemma dqst_auth_write_bot v γglob era ca l t b :
-    dqst_auth γglob era ca l t b -∗
-    dqst_auth γglob era ca (mod_set l b v) t b.
+  Lemma dqst_auth_write_bot v γdqst era ca l t b :
+    dqst_auth γdqst era ca l t b -∗
+    dqst_auth γdqst era ca (mod_set l b v) t b.
   Proof.
-    desγ γglob.
+    desγ γdqst.
     iIntros "Auth".
       iDestruct "Auth" as (γtbeO) "(%HltO & tbO & eltO & museO)".
       iDestruct "eltO" as (elts) "[Elts %Heltslen]".
@@ -538,12 +537,12 @@ Section dqst.
     apply neq_symm, close_mod_neq; lia.
   Qed.
 
-  Lemma dqst_auth_update γglob era ca l t b :
+  Lemma dqst_auth_update γdqst era ca l t b :
     t < b →
-    dqst_auth γglob era ca l t b ==∗
-    dqst_auth γglob era ca l (S t) b.
+    dqst_auth γdqst era ca l t b ==∗
+    dqst_auth γdqst era ca l (S t) b.
   Proof with extended_auto.
-    desγ γglob.
+    desγ γdqst.
     iIntros (Hlt) "Auth".
       iDestruct "Auth" as (γtbeO) "(%HltO & [tbO tbeO] & eltO & museO)".
       iDestruct "eltO" as (elts) "[Elts %Heltslen]".
@@ -563,12 +562,12 @@ Section dqst.
     replace (S t - length elts) with 0; simpl... fr.
   Qed.
 
-  Lemma dqst_auth_push γglob era ca l t b :
+  Lemma dqst_auth_push γdqst era ca l t b :
     S b < t + length l →
-    dqst_auth γglob era ca l t b ==∗
-    dqst_auth γglob era ca l t (S b).
+    dqst_auth γdqst era ca l t b ==∗
+    dqst_auth γdqst era ca l t (S b).
   Proof with extended_auto.
-    desγ γglob.
+    desγ γdqst.
     iIntros (Hlt) "Auth".
       iDestruct "Auth" as (γtbeO) "(%HltO & [tbO tbeO] & eltO & museO)".
       iDestruct "eltO" as (elts) "[Elts %Heltslen]".
@@ -588,12 +587,12 @@ Section dqst.
     replace (t - length elts) with 0; simpl... fr.
   Qed.
 
-  Lemma dqst_auth_pop γglob era ca l t b :
+  Lemma dqst_auth_pop γdqst era ca l t b :
     t < b - 1 →
-    dqst_auth γglob era ca l t b ==∗
-    dqst_auth γglob era ca l t (b - 1).
+    dqst_auth γdqst era ca l t b ==∗
+    dqst_auth γdqst era ca l t (b - 1).
   Proof with extended_auto.
-    desγ γglob.
+    desγ γdqst.
     iIntros (Hlt) "Auth".
       iDestruct "Auth" as (γtbeO) "(%HltO & [tbO tbeO] & eltO & museO)".
       iDestruct "eltO" as (elts) "[Elts %Heltslen]".
@@ -602,15 +601,15 @@ Section dqst.
     iModIntro. fr. fr. case_bool_decide...
   Qed.
 
-  Lemma dqst_auth_archive ca' l' γglob era ca l t b :
+  Lemma dqst_auth_archive ca' l' γdqst era ca l t b :
     length l ≤ length l' →
     circ_slice l t b = circ_slice l' t b →
     ca ↦∗ l -∗
-    dqst_auth γglob era ca l t b ==∗
-    dqst_archived γglob era ca l t b ∗
-    dqst_auth γglob (S era) ca' l' t b.
+    dqst_auth γdqst era ca l t b ==∗
+    dqst_archived γdqst era ca l t b ∗
+    dqst_auth γdqst (S era) ca' l' t b.
   Proof with extended_auto.
-    desγ γglob.
+    desγ γdqst.
     iIntros (Hlong Heqs) "Own Auth".
       iDestruct "Auth" as (γtbeO) "(%HltO & [tbO tbeO] & eltO & museO)".
       iDestruct "eltO" as (elts) "[Elts %Heltslen]".
@@ -666,66 +665,52 @@ Section proof.
   Context `{!heapGS Σ, !dequeG Σ, !circleG Σ} (N : namespace).
   Notation iProp := (iProp Σ).
 
-  Definition deque_inv (γq γpop γera : gname) (γglob : glob_gnames)
+  Definition deque_inv (γq γera : gname) (γdqst : dqst_gnames)
   (C top bot : loc) : iProp :=
-    ∃ (era : nat) (arr : loc) (l : list val) (t b : nat),
+    ∃ (era : nat) (arr : loc) (l : list val) (t b : nat) (pop : bool),
       ⌜1 ≤ t ≤ b ∧ b < t + length l ∧ length l ≠ 0⌝ ∗
-      (* abstract states *)
-      ( dqst_auth γglob era arr l t b ∗
-        own γq (●E (circ_slice l t b)) ∗
-        ghost_var γera (1/2) (era, l)
-      ) ∗
-      (* circular array *)
-      ( C ↦{#1/2} (#arr, #(length l)) ∗
-        arr ↦∗{#1/2} l
-      ) ∗
-      (* top *)
+      (* abstract *)
+      own γq (●E (circ_slice l t b)) ∗
+      ghost_var γera (1/2) (era, arr, l, b, pop) ∗
+      dqst_auth γdqst era arr l t b ∗
+      (* physical *)
+      C ↦{#1/2} (#arr, #(length l)) ∗
+      arr ↦∗{#1/2} l ∗
       top ↦ #t ∗
-      (* bottom *)
-      ( ∃ (Popping : bool),
-        let bp := if Popping then b-1 else b in
-        bot ↦{#1/2} #bp ∗
-        ghost_var γpop (1/2) Popping
-      ).
+      bot ↦{#1/2} #(if pop then b-1 else b).
 
   Definition is_deque (γ : gname) (q : val) : iProp :=
-    ∃ (γq γpop γera : gname) (γglob : glob_gnames) (C top bot : loc),
+    ∃ (γq γera : gname) (γdqst : dqst_gnames) (C top bot : loc),
       ⌜q = (#C, #top, #bot)%V⌝ ∗
-      ⌜γ = encode (γq, γpop, γera, γglob)⌝ ∗
-      inv N (deque_inv γq γpop γera γglob C top bot).
+      ⌜γ = encode (γq, γera, γdqst)⌝ ∗
+      inv N (deque_inv γq γera γdqst C top bot).
   Global Instance is_deque_persistent γ q :
     Persistent (is_deque γ q) := _.
 
   Definition deque_content (γ : gname) (frag : list val) : iProp :=
-    ∃ (γq γpop γera : gname) (γglob : glob_gnames),
-      ⌜γ = encode (γq, γpop, γera, γglob)⌝ ∗
+    ∃ (γq γera : gname) (γdqst : dqst_gnames),
+      ⌜γ = encode (γq, γera, γdqst)⌝ ∗
       own γq (◯E frag).
   Global Instance deque_content_timeless γ frag :
     Timeless (deque_content γ frag) := _.
 
   (* owner of the deque who can call push and pop *)
   Definition own_deque (γ : gname) (q : val) : iProp :=
-    ∃ (γq γpop γera : gname) (γglob : glob_gnames) (era : nat)
+    ∃ (γq γera : gname) (γdqst : dqst_gnames) (era : nat)
     (l : list val) (C arr top bot : loc) (b : nat),
-      ⌜γ = encode (γq, γpop, γera, γglob)⌝ ∗
+      ⌜γ = encode (γq, γera, γdqst)⌝ ∗
       ⌜q = (#C, #top, #bot)%V⌝ ∗
-      (* array state *)
-      ghost_var γera (1/2) (era, l) ∗
-      (* own circle *)
-      ( C ↦{#1/2} (#arr, #(length l)) ∗
-        arr ↦∗{#1/2} l
-      ) ∗
-      (* own bottom *)
-      ( bot ↦{#1/2} #b ∗
-        ghost_var γpop (1/2) false
-      ).
+      ghost_var γera (1/2) (era, arr, l, b, false) ∗
+      C ↦{#1/2} (#arr, #(length l)) ∗
+      arr ↦∗{#1/2} l ∗
+      bot ↦{#1/2} #b.
   
   Lemma deque_content_exclusive γ frag1 frag2 :
     deque_content γ frag1 -∗ deque_content γ frag2 -∗ False.
   Proof.
     iIntros "C1 C2".
-      iDestruct "C1" as (γq γpop γera γglob) "[%Enc C1]".
-      iDestruct "C2" as (γq' γpop' γera' γglob') "[%Enc' C2]".
+      iDestruct "C1" as (γq γera γdqst) "[%Enc C1]".
+      iDestruct "C2" as (γq' γera' γdqst') "[%Enc' C2]".
       encode_agree Enc.
     by iDestruct (own_valid_2 with "C1 C2") as %?%auth_frag_op_valid_1.
   Qed.
@@ -760,21 +745,19 @@ Section proof.
     (* allocate *)
     wp_alloc arr as "[arr↦1 arr↦2]"... wp_pures.
     wp_alloc bot as "[b↦1 b↦2]". wp_alloc top as "t↦".
-    wp_alloc A as "[A↦1 A↦2]". wp_pures.
+    wp_alloc C as "[C↦1 C↦2]". wp_pures.
 
     (* make resources *)
-    iMod (own_alloc (●E [] ⋅ ◯E [])) as (γq) "[γq● γq◯]".
-      1: apply excl_auth_valid.
-    iMod (ghost_var_alloc false) as (γpop) "[γpop1 γpop2]".
-    iMod (dqst_auth_alloc arr (replicate n #0)) as (γglob) "Auth"...
-    iMod (ghost_var_alloc (0, replicate n #0)) as (γera) "[eraG1 eraG2]".
-    iMod (inv_alloc N _ (deque_inv γq γpop γera γglob A top bot)
-      with "[A↦1 t↦ b↦1 arr↦1 γq● γpop1 Auth eraG1]") as "Inv".
-    { fr. fr. fr. }
+    iMod (own_alloc (●E [] ⋅ ◯E [])) as (γq) "[γq● γq◯]". 1: apply excl_auth_valid.
+    iMod (ghost_var_alloc (0, arr, (replicate n #0), 1, false)) as (γera) "[Era1 Era2]".
+    iMod (dqst_auth_alloc arr (replicate n #0)) as (γdqst) "Auth"...
+    iMod (inv_alloc N _ (deque_inv γq γera γdqst C top bot)
+      with "[C↦1 t↦ b↦1 arr↦1 γq● Auth Era1]") as "Inv".
+    { fr. fr. }
 
     (* apply Φ *)
     iApply "HΦ". iModIntro. iSplitL "Inv"; first fr.
-    iSplitL "γq◯"; fr. fr. instantiate (1:=1)...
+    iSplitL "γq◯"; fr. fr.
   Qed.
 
   Lemma push_spec γ q (v : val) :
@@ -786,11 +769,11 @@ Section proof.
       RET #(), own_deque γ q >>>.
   Proof with extended_auto.
     iIntros "#Is Own" (Φ) "AU".
-      iDestruct "Own" as (γq γpop γera γglob) "Own".
+      iDestruct "Own" as (γq γera γdqst) "Own".
         iDestruct "Own" as (era l C arr top bot b) "Own".
-        iDestruct "Own" as "(%Enc & %Q & eraOwn & [COwn AOwn] & [bOwn popOwn])".
+        iDestruct "Own" as "(%Enc & %Q & eraOwn & COwn & AOwn & bOwn)".
         subst q.
-      iDestruct "Is" as (γq' γpop' γera' γglob') "Inv".
+      iDestruct "Is" as (γq' γera' γdqst') "Inv".
         iDestruct "Inv" as (C' top' bot') "Inv".
         iDestruct "Inv" as "(%Q & %Enc' & Inv)".
         injection Q as [= <- <- <-]. encode_agree Enc.
@@ -799,229 +782,132 @@ Section proof.
 
     (* 1. load top *)
     wp_bind (! _)%E.
-      iInv "Inv" as (era1 arr1 l1 t1 b1) "Invs".
-        iDestruct "Invs" as "(>%Htb1 & >Abst & >A & >Top & >Bot)".
-      iDestruct "A" as "[C↦ arr↦]".
-        iDestruct (mapsto_agree with "COwn C↦") as "%Hl1". injection Hl1 as [= <- Hlen].
-        iDestruct (array_agree with "AOwn arr↦") as "%"... subst l1. clear Hlen.
-      iCombine "C↦ arr↦" as "A".
-      iDestruct "Bot" as (Pop1) "[bot↦ pop]".
-        iDestruct (ghost_var_agree with "popOwn pop") as "%". subst Pop1.
-        iDestruct (mapsto_agree with "bOwn bot↦") as "%Hb".
-        injection Hb as [= Hb]. assert (b = b1)... subst b1. clear Hb.
-      iCombine "bot↦ pop" as "Bot".
-      iDestruct "Abst" as "(Glob & ● & Era)".
-        iDestruct (dqst_get_frag with "Glob") as "#F1".
-      iCombine "Glob ● Era" as "Abst".
+      iInv "Inv" as (era1 arr1 l1 t1 b1 pop1) ">Invs".
+        iDestruct "Invs" as "(%Htb1 & ● & Era & Dqst & C & A & T & B)".
+      iDestruct (ghost_var_agree with "eraOwn Era") as "%Eq"; injection Eq as [= <- <- <- <- <-].
+      iDestruct (dqst_get_frag with "Dqst") as "#F1".
       wp_load.
-      iModIntro. iSplitL "Abst A Top Bot".
-      { iExists _,_,l. fr. fr. instantiate (1:=false)... }
+    iModIntro. iSplitL "● Era Dqst C A T B".
+    { iExists _,_,l. fr. }
     wp_pures. wp_load. wp_pures.
     
     case_bool_decide; last first; wp_pures.
     - (* 2. write to circle *)
-      wp_load. wp_pures.
+      wp_load. wp_pures. rewrite rem_mod_eq...
       wp_bind (_ <- _)%E.
-        iInv "Inv" as (era2 arr2 l2 t2 b2) "Invs".
-          iDestruct "Invs" as "(>%Htb2 & >Abst & >A & >Top & >Bot)".
-        iDestruct "A" as "[C↦ arr↦]".
-          iDestruct (mapsto_agree with "COwn C↦") as "%Hl2". injection Hl2 as [= <- Hlen].
-          iDestruct (array_agree with "AOwn arr↦") as "%"... subst l2. clear Hlen.
-          iCombine "AOwn arr↦" as "arr↦".
-          rewrite rem_mod_eq...
-          iApply (wp_store_offset with "[arr↦]")... 1: apply mod_get_is_Some...
-          iNext. iIntros "arr↦".
-          iDestruct "arr↦" as "[AOwn arr↦]".
-        iCombine "C↦ arr↦" as "A".
-        iDestruct "Bot" as (Pop2) "[bot↦ pop]".
-          iDestruct (ghost_var_agree with "popOwn pop") as "%". subst Pop2.
-          iDestruct (mapsto_agree with "bOwn bot↦") as "%Hb".
-          injection Hb as [= Hb]. assert (b = b2)... subst b2.
-        iCombine "bot↦ pop" as "Bot".
-        iDestruct "Abst" as "(Glob & ● & Era)".
-          iDestruct (dqst_auth_write_bot v with "Glob") as "Glob"...
-          iDestruct (ghost_var_agree with "eraOwn Era") as "%Hera2".
-          injection Hera2 as [= <-].
-          iMod (ghost_var_update_2 (era, mod_set l b v) with "eraOwn Era") as "[eraOwn Era]"...
-        iCombine "Glob ● Era" as "Abst".
-      iModIntro. iSplitL "Abst A Top Bot".
+        iInv "Inv" as (era2 arr2 l2 t2 b2 pop2) ">Invs".
+          iDestruct "Invs" as "(%Htb2 & ● & Era & Dqst & C & A & T & B)".
+        iDestruct (ghost_var_agree with "eraOwn Era") as "%Eq"; injection Eq as [= <- <- <- <- <-].
+        iMod (ghost_var_update_halves (era, arr, (mod_set l b v), b, false)
+          with "eraOwn Era") as "[eraOwn Era]".
+        iDestruct (dqst_auth_write_bot v with "Dqst") as "Dqst".
+        iCombine "AOwn A" as "A".
+          iApply (wp_store_offset with "A"). 1: apply mod_get_is_Some...
+        iIntros "!> [AOwn A]".
+      iModIntro. iSplitL "● Era Dqst C A T B".
       { iExists _,_,(mod_set l b v),t2,b.
-        rewrite mod_set_length circ_slice_update_right...
-        fr. iExists false... }
+        rewrite mod_set_length circ_slice_update_right... fr. }
       wp_pures.
 
       (* 3. increment bot *)
-      iInv "Inv" as (era3 arr3 l3 t3 b3) "Invs".
-        iDestruct "Invs" as "(>%Htb4 & >Abst & A & >Top & >Bot)".
-        iDestruct "Bot" as (Pop3) "[bot↦ pop]".
-          iDestruct (ghost_var_agree with "pop popOwn") as "%Eq". subst Pop3.
-          iDestruct (mapsto_agree with "bOwn bot↦") as "%Eq".
-            injection Eq as [= Hb3]. assert (b = b3)... subst b3. clear Hb3.
-          iCombine "bOwn bot↦" as "bot↦".
-            wp_store. replace (Z.of_nat b + 1)%Z with (Z.of_nat (S b))...
-          iDestruct "bot↦" as "[bOwn bot↦]".
-        iCombine "bot↦ pop" as "Bot".
-        iDestruct "Abst" as "(Glob & ● & Era)".
-          iDestruct (dqst_get_lb with "Glob F1") as "%Ht14".
-          iDestruct (ghost_var_agree with "eraOwn Era") as "%Eq".
-          injection Eq as [= <- <-].
-        iCombine "Glob ● Era" as "Abst".
-        iDestruct "A" as "[C↦ arr↦]".
-          iDestruct (mapsto_agree with "COwn C↦") as "%Hl3". injection Hl3 as [= <- Hlen].
-          iDestruct (array_agree with "AOwn arr↦") as "%Hl3".
-          1: rewrite insert_length...
-        iCombine "C↦ arr↦" as "A".
+      iInv "Inv" as (era3 arr3 l3 t3 b3 pop3) ">Invs".
+        iDestruct "Invs" as "(%Htb3 & ● & Era & Dqst & C & A & T & B)".
+        iDestruct (ghost_var_agree with "eraOwn Era") as "%Eq"; injection Eq as [= <- <- <- <- <-].
+        iMod (ghost_var_update_halves (era, arr, (mod_set l b v), S b, false)
+          with "eraOwn Era") as "[eraOwn Era]".
+        iDestruct (dqst_get_lb with "Dqst F1") as "%Ht13".
+          iMod (dqst_auth_push with "Dqst") as "Dqst". 1: rewrite mod_set_length...
+        iCombine "bOwn B" as "B". wp_store.
+          replace (Z.of_nat b + 1)%Z with (Z.of_nat (S b))...
+        iDestruct "B" as "[bOwn B]".
       iMod "AU" as (l') "[Cont [_ Commit]]".
-        iDestruct "Cont" as (γq' γpop' γera' γbglob') "[%Enc' ◯]".
-          encode_agree Enc.
-        iDestruct "Abst" as "(Glob & ● & Era)".
-          iMod (dqst_auth_push with "Glob") as "Glob".
-            1: rewrite insert_length...
-          iDestruct (own_ea_agree with "● ◯") as "%Hl'".
-          iMod (own_ea_update (l' ++ [v]) with "● ◯") as "[● ◯]".
-        iCombine "Glob ● Era" as "Abst".
-      iMod ("Commit" with "[◯]") as "HΦ". 1: fr.
-      
-      iModIntro.
-      iSplitL "A Abst Top Bot".
+        iDestruct "Cont" as (γq' γera' γbglob') "[%Enc' ◯]". encode_agree Enc.
+        iDestruct (own_ea_agree with "● ◯") as "%Hl'".
+        iMod (own_ea_update (l' ++ [v]) with "● ◯") as "[● ◯]".
+        iMod ("Commit" with "[◯]") as "HΦ". 1: fr.
+      iModIntro. iSplitL "● Era Dqst C A T B".
       { iExists era, arr, (mod_set l b v), t3, (S b). fr.
-        rewrite (circ_slice_extend_right _ _ _ v)...
-        2: rewrite mod_set_get... subst l'.
-        fr. iExists false...
-      }
+        rewrite (circ_slice_extend_right _ _ _ v)... 2: rewrite mod_set_get...
+        subst l'. fr. rewrite mod_set_length... }
       iApply "HΦ".
-        iExists γq, γpop, γera, γglob.
+        iExists γq, γera, γdqst.
         iExists era, (mod_set l b v), C, arr, top, bot, (S b).
         fr. rewrite insert_length...
     - (* X. grow *)
       wp_bind (grow_circle _ _ _)%E.
-      awp_apply (grow_circle_spec with "[eraOwn COwn AOwn bOwn popOwn AU]")...
-        iInv "Inv" as (eraX arrX lX tX bX) "Invs".
-          iDestruct "Invs" as "(>%HtbX & >Abst & >A & >Top & >Bot)".
-        iDestruct "Abst" as "(Glob & ● & Era)".
-          iDestruct (ghost_var_agree with "eraOwn Era") as "%Eq".
-          injection Eq as [= <- <-].
-        iCombine "Glob ● Era" as "Abst".
-        iDestruct "A" as "[C↦ arr↦]".
-          iDestruct (mapsto_agree with "COwn C↦") as "%HlX".
-          injection HlX as [= <-].
-          iCombine "AOwn arr↦" as "arr↦".
-          iAaccIntro with "arr↦".
-          { iIntros "arr↦". iDestruct "arr↦" as "[AOwn arr↦]".
-            iCombine "C↦ arr↦" as "A".
-            iSplitL "Abst A Top Bot". 2: fr. iExists _,_,l. fr. }
-          iIntros (arrX lX) "(%HlenX & %Heqs & arr↦)".
-          iDestruct "arr↦" as "[AOwn arr↦]".
-        iCombine "C↦ arr↦" as "A".
-      iModIntro. iSplitL "Abst A Top Bot".
+      awp_apply (grow_circle_spec with "[eraOwn COwn AOwn bOwn AU]")...
+        iInv "Inv" as (eraX arrX lX tX bX popX) ">Invs".
+          iDestruct "Invs" as "(%HtbX & ● & Era & Dqst & C & A & T & B)".
+        iDestruct (ghost_var_agree with "eraOwn Era") as "%Eq"; injection Eq as [= <- <- <- <- <-].
+        iCombine "AOwn A" as "A".
+          iAaccIntro with "A".
+          { iIntros "[AOwn A]". iSplitL "● Era Dqst C A T B". 2: fr.
+            iExists _,_,l. fr. }
+        iIntros (arrX lX) "(%HlenX & %Heqs & [AOwn A])".
+      iModIntro. iSplitL "● Era Dqst C A T B".
       { iExists _,_,l. fr. }
-      iIntros "arrX↦". wp_pures.
+      iIntros "AX". wp_pures.
 
       (* Y. replace array *)
       wp_bind (_ <- _)%E.
-        iInv "Inv" as (eraY caY lY tY bY) "Invs".
-          iDestruct "Invs" as "(>%HtbY & >Abst & >A & >Top & >Bot)".
-        iDestruct "A" as "[C↦ arr↦]".
-          iDestruct (mapsto_agree with "COwn C↦") as "%HlY".
-          injection HlY as [= <- HlY]. rewrite -HlY.
-          iCombine "COwn C↦" as "C↦". wp_store.
-          iDestruct "C↦" as "[COwn C↦]".
-        (*iCombine "C↦ arr↦" as "A".*)
-        iDestruct "Bot" as (PopY) "[bot↦ pop]".
-          iDestruct (ghost_var_agree with "pop popOwn") as "%Eq". subst PopY.
-          iDestruct (mapsto_agree with "bOwn bot↦") as "%Eq".
-            injection Eq as [= HbY]. assert (b = bY)... subst bY. clear HbY.
-        iCombine "bot↦ pop" as "Bot".
-        iDestruct "Abst" as "(Glob & ● & Era)".
-          iDestruct (dqst_get_lb with "Glob F1") as "%Ht1Y".
-          apply (circ_slice_split_eq tY) in Heqs as [_ HeqsY]...
-          iDestruct (ghost_var_agree with "eraOwn Era") as "%Eq".
-          injection Eq as [= <- <-].
-          iCombine "AOwn arr↦" as "arr↦".
-          iMod (dqst_auth_archive arrX lX with "arr↦ Glob") as "[#Arch Glob]"...
-          iMod (ghost_var_update_2 (S era, lX) with "eraOwn Era") as "[eraOwn Era]"...
-        iCombine "Glob ● Era" as "Abst".
-      iDestruct "arrX↦" as "[AOwn arr↦]".
-      iCombine "C↦ arr↦" as "A".
-      replace (circ_slice l tY b) with (circ_slice lX tY b); last first.
-
-      iSplitL "A Abst Top Bot".
+        iInv "Inv" as (eraY caY lY tY bY popY) ">Invs".
+          iDestruct "Invs" as "(%HtbY & ● & Era & Dqst & C & A & T & B)".
+        iDestruct (ghost_var_agree with "eraOwn Era") as "%Eq"; injection Eq as [= <- <- <- <- <-].
+        iMod (ghost_var_update_halves (S era, arrX, lX, b, false)
+          with "eraOwn Era") as "[eraOwn Era]".
+          iDestruct (dqst_get_lb with "Dqst F1") as "%Ht1Y".
+          apply (circ_slice_split_eq tY) in Heqs as Heqsd... destruct Heqsd as [_ HeqsR]...
+        iCombine "AOwn A" as "A".
+          iMod (dqst_auth_archive arrX lX with "[A] [Dqst]") as "[#Arch Dqst]".
+          2: apply HeqsR. all: eauto. 1: fr.
+          iDestruct "AX" as "[AOwn A]".
+        iCombine "COwn C" as "C". wp_store.
+        iDestruct "C" as "[COwn C]".
+      iSplitL "● Era Dqst C A T B".
       { iModIntro; iNext. iExists _,_,lX.
-        fr. fr. instantiate (1:=false)... }
+        fr. fr. rewrite -HeqsR... }
       iModIntro. wp_pures. wp_load. wp_pures.
 
       (* 2. write to circle *)
+      rewrite rem_mod_eq...
       wp_bind (_ <- _)%E.
-        iInv "Inv" as (era2 arr2 l2 t2 b2) "Invs".
-          iDestruct "Invs" as "(>%Htb2 & >Abst & >A & >Top & >Bot)".
-        iDestruct "A" as "[C↦ arr↦]".
-          iDestruct (mapsto_agree with "COwn C↦") as "%Hl2". injection Hl2 as [= <- Hlen].
-          iDestruct (array_agree with "AOwn arr↦") as "%"... subst l2. clear Hlen.
-          iCombine "AOwn arr↦" as "arr↦".
-          rewrite rem_mod_eq...
-          iApply (wp_store_offset with "[arr↦]")... 1: apply mod_get_is_Some...
-          iNext. iIntros "arr↦".
-          iDestruct "arr↦" as "[AOwn arr↦]".
-        iCombine "C↦ arr↦" as "A".
-        iDestruct "Bot" as (Pop2) "[bot↦ pop]".
-          iDestruct (ghost_var_agree with "popOwn pop") as "%". subst Pop2.
-          iDestruct (mapsto_agree with "bOwn bot↦") as "%Hb".
-          injection Hb as [= Hb]. assert (b = b2)... subst b2.
-        iCombine "bot↦ pop" as "Bot".
-        iDestruct "Abst" as "(Glob & ● & Era)".
-          iDestruct (dqst_auth_write_bot v with "Glob") as "Glob"...
-          iDestruct (ghost_var_agree with "eraOwn Era") as "%Hera2".
-          injection Hera2 as [= <-].
-          iMod (ghost_var_update_2 (S era, mod_set lX b v) with "eraOwn Era") as "[eraOwn Era]"...
-        iCombine "Glob ● Era" as "Abst".
-      iModIntro. iSplitL "Abst A Top Bot".
+        iInv "Inv" as (era2 arr2 l2 t2 b2 pop2) ">Invs".
+          iDestruct "Invs" as "(%Htb2 & ● & Era & Dqst & C & A & T & B)".
+        iDestruct (ghost_var_agree with "eraOwn Era") as "%Eq"; injection Eq as [= <- <- <- <- <-].
+        iMod (ghost_var_update_halves (S era, arrX, (mod_set lX b v), b, false)
+          with "eraOwn Era") as "[eraOwn Era]".
+        iDestruct (dqst_auth_write_bot v with "Dqst") as "Dqst".
+        iCombine "AOwn A" as "A".
+          iApply (wp_store_offset with "A"). 1: apply mod_get_is_Some...
+        iIntros "!> [AOwn A]".
+      iModIntro. iSplitL "● Era Dqst C A T B".
       { iExists _,_,(mod_set lX b v),t2,b.
-        rewrite mod_set_length circ_slice_update_right...
-        fr. iExists false... }
+        rewrite mod_set_length circ_slice_update_right... fr. }
       wp_pures.
 
       (* 3. increment bot *)
-      iInv "Inv" as (era3 arr3 l3 t3 b3) "Invs".
-        iDestruct "Invs" as "(>%Htb4 & >Abst & A & >Top & >Bot)".
-        iDestruct "Bot" as (Pop3) "[bot↦ pop]".
-          iDestruct (ghost_var_agree with "pop popOwn") as "%Eq". subst Pop3.
-          iDestruct (mapsto_agree with "bOwn bot↦") as "%Eq".
-            injection Eq as [= Hb3]. assert (b = b3)... subst b3. clear Hb3.
-          iCombine "bOwn bot↦" as "bot↦".
-            wp_store. replace (Z.of_nat b + 1)%Z with (Z.of_nat (S b))...
-          iDestruct "bot↦" as "[bOwn bot↦]".
-        iCombine "bot↦ pop" as "Bot".
-        iDestruct "Abst" as "(Glob & ● & Era)".
-          iDestruct (dqst_get_lb with "Glob F1") as "%Ht14".
-          iDestruct (ghost_var_agree with "eraOwn Era") as "%Eq".
-          injection Eq as [= <- <-].
-        iCombine "Glob ● Era" as "Abst".
-        iDestruct "A" as "[C↦ arr↦]".
-          iDestruct (mapsto_agree with "COwn C↦") as "%Hl3". injection Hl3 as [= <- Hlen].
-          iDestruct (array_agree with "AOwn arr↦") as "%Hl3".
-          1: rewrite insert_length...
-        iCombine "C↦ arr↦" as "A".
+      iInv "Inv" as (era3 arr3 l3 t3 b3 pop3) ">Invs".
+        iDestruct "Invs" as "(%Htb3 & ● & Era & Dqst & C & A & T & B)".
+        iDestruct (ghost_var_agree with "eraOwn Era") as "%Eq"; injection Eq as [= <- <- <- <- <-].
+        iMod (ghost_var_update_halves (S era, arrX, (mod_set lX b v), S b, false)
+          with "eraOwn Era") as "[eraOwn Era]".
+        iDestruct (dqst_get_lb with "Dqst F1") as "%Ht13".
+          iMod (dqst_auth_push with "Dqst") as "Dqst". 1: rewrite mod_set_length...
+        iCombine "bOwn B" as "B". wp_store.
+          replace (Z.of_nat b + 1)%Z with (Z.of_nat (S b))...
+        iDestruct "B" as "[bOwn B]".
       iMod "AU" as (l') "[Cont [_ Commit]]".
-        iDestruct "Cont" as (γq' γpop' γera' γbglob') "[%Enc' ◯]".
-          encode_agree Enc.
-        iDestruct "Abst" as "(Glob & ● & Era)".
-          iMod (dqst_auth_push with "Glob") as "Glob".
-            1: rewrite insert_length...
-          iDestruct (own_ea_agree with "● ◯") as "%Hl'".
-          iMod (own_ea_update (l' ++ [v]) with "● ◯") as "[● ◯]".
-        iCombine "Glob ● Era" as "Abst".
-      iMod ("Commit" with "[◯]") as "HΦ". 1: fr.
-      
-      iModIntro.
-      iSplitL "A Abst Top Bot".
-      { iExists (S era), arrX, (mod_set lX b v), t3, (S b). fr.
-        rewrite (circ_slice_extend_right _ _ _ v)...
-        2: rewrite mod_set_get... subst l'.
-        fr. iExists false...
-      }
+        iDestruct "Cont" as (γq' γera' γbglob') "[%Enc' ◯]". encode_agree Enc.
+        iDestruct (own_ea_agree with "● ◯") as "%Hl'".
+        iMod (own_ea_update (l' ++ [v]) with "● ◯") as "[● ◯]".
+        iMod ("Commit" with "[◯]") as "HΦ". 1: fr.
+      iModIntro. iSplitL "● Era Dqst C A T B".
+      { iExists (S era), arrX, (mod_set lX b v), t3, (S b), false. fr.
+        1: rewrite mod_set_length... subst l'.
+        rewrite (circ_slice_extend_right _ _ _ v)... rewrite mod_set_get... }
       iApply "HΦ".
-        iExists γq, γpop, γera, γglob.
-        iExists _,(mod_set lX b v). fr. fr. rewrite insert_length...
+        iExists γq, γera, γdqst.
+        iExists (S era), (mod_set lX b v). fr. fr. rewrite insert_length...
     Unshelve. done.
   Qed.
 
@@ -1040,11 +926,11 @@ Section proof.
       RET ov, own_deque γ q >>>.
   Proof with extended_auto.
     iIntros "#Is Own" (Φ) "AU".
-      iDestruct "Own" as (γq γpop γera γglob) "Own".
+      iDestruct "Own" as (γq γera γdqst) "Own".
         iDestruct "Own" as (era l C arr top bot b) "Own".
-        iDestruct "Own" as "(%Enc & %Q & eraOwn & [COwn AOwn] & [bOwn popOwn])".
+        iDestruct "Own" as "(%Enc & %Q & eraOwn & COwn & AOwn & bOwn)".
         subst q.
-      iDestruct "Is" as (γq' γpop' γera' γglob') "Inv".
+      iDestruct "Is" as (γq' γera' γdqst') "Inv".
         iDestruct "Inv" as (C' top' bot') "Inv".
         iDestruct "Inv" as "(%Q & %Enc' & Inv)".
         injection Q as [= <- <- <-]. encode_agree Enc.
@@ -1053,216 +939,144 @@ Section proof.
 
     (* 1. decrement bot *)
     wp_bind (_ <- _)%E.
-      iInv "Inv" as (era1 ca1 l1 t1 b1) "Invs".
-        iDestruct "Invs" as "(>%Htb1 & >Abst & >A & >Top & >Bot)".
-      iDestruct "Abst" as "(Glob & Q & Era)".
-        iDestruct (ghost_var_agree with "eraOwn Era") as "%Eq".
-        injection Eq as [= <- <-].
-      iCombine "Glob Q Era" as "Abst".
-      iDestruct "A" as "[C↦ arr↦]".
-        iDestruct (mapsto_agree with "COwn C↦") as "%Hl1". injection Hl1 as [= <-].
-      iCombine "C↦ arr↦" as "A".
-      iDestruct "Bot" as (Pop1) "[bot↦ pop]".
-        iDestruct (ghost_var_agree with "pop popOwn") as "%". subst Pop1.
-        iMod (ghost_var_update_2 true with "pop popOwn") as "[pop popOwn]"...
-        iDestruct (mapsto_agree with "bot↦ bOwn") as "%Eq".
-        injection Eq as [= Eq]. assert (b = b1)... subst b1. clear Eq.
-        iCombine "bot↦ bOwn" as "bot↦". wp_store.
-          replace (Z.of_nat b - 1)%Z with (Z.of_nat (b - 1))%Z...
-        iDestruct "bot↦" as "[bot↦ bOwn]".
-      iCombine "bot↦ pop" as "Bot".
-    iModIntro. iSplitL "Abst A Top Bot".
-    { iExists _,_,l. fr. fr. instantiate (1:=true)... }
+      iInv "Inv" as (era1 ca1 l1 t1 b1 pop1) ">Invs".
+        iDestruct "Invs" as "(%Htb1 & ● & Era & Dqst & C & A & T & B)".
+      iDestruct (ghost_var_agree with "eraOwn Era") as "%Eq"; injection Eq as [= <- <- <- <- <-].
+      iMod (ghost_var_update_halves (era, arr, l, b, true)
+        with "eraOwn Era") as "[eraOwn Era]".
+      iCombine "bOwn B" as "B". wp_store.
+      iDestruct "B" as "[bOwn B]".
+    iModIntro. iSplitL "● Era Dqst C A T B".
+    { iExists _,_,l. fr. }
     wp_pures.
 
     (* 2. load top *)
     wp_bind (! _)%E.
-      iInv "Inv" as (era2 ca2 l2 t2 b2) "Invs".
-        iDestruct "Invs" as "(>%Htb2 & >Abst & >A & >Top & >Bot)".
-      iDestruct "Abst" as "(Glob & Q & Era)".
-        iDestruct (ghost_var_agree with "eraOwn Era") as "%Eq".
-        injection Eq as [= <- <-].
-      iCombine "Glob Q Era" as "Abst".
-      iDestruct "A" as "[C↦ arr↦]".
-        iDestruct (mapsto_agree with "COwn C↦") as "%Hl1". injection Hl1 as [= <-].
-      iCombine "C↦ arr↦" as "A".
-      iDestruct "Bot" as (Pop2) "[bot↦ pop]".
-        iDestruct (ghost_var_agree with "pop popOwn") as "%". subst Pop2.
-        iDestruct (mapsto_agree with "bot↦ bOwn") as "%Eq".
-        injection Eq as [= Eq]. assert (b = b2)... subst b2. clear Eq.
-      iCombine "bot↦ pop" as "Bot".
+      iInv "Inv" as (era2 ca2 l2 t2 b2 pop2) ">Invs".
+        iDestruct "Invs" as "(%Htb2 & ● & Era & Dqst & C & A & T & B)".
+      iDestruct (ghost_var_agree with "eraOwn Era") as "%Eq"; injection Eq as [= <- <- <- <- <-].
       wp_load.
-    
+
     destruct (decide (t2 < b-1)).
     { (* normal case, this point is the commit point *)
       iMod "AU" as (l') "[Cont [_ Commit]]".
-        iDestruct "Cont" as (γq' γpop' γera' γglob') "[%Enc' ◯]".
-          encode_agree Enc.
+        iDestruct "Cont" as (γq' γera' γdqst') "[%Enc' ◯]". encode_agree Enc.
         destruct (mod_get_is_Some l (b-1)) as [x Hx]...
-        iDestruct "Abst" as "(Glob & Q & Era)".
-          iMod (dqst_auth_pop with "Glob") as "Glob"...
-          iDestruct (own_ea_agree with "Q ◯") as "%Eq". subst l'.
-          iMod (own_ea_update (circ_slice l t2 (b-1)) with "Q ◯") as "[Q ◯]".
-        iCombine "Glob Q Era" as "Abst".
-        iDestruct "Bot" as "[bot↦ pop]".
-          iMod (ghost_var_update_2 false with "pop popOwn") as "[pop popOwn]"...
-        iCombine "bot↦ pop" as "Bot".
+        iDestruct (own_ea_agree with "● ◯") as "%Eq". subst l'.
+        iMod (own_ea_update (circ_slice l t2 (b-1)) with "● ◯") as "[● ◯]".
+        iMod (ghost_var_update_halves (era, arr, l, b-1, false)
+          with "eraOwn Era") as "[eraOwn Era]".
+        iMod (dqst_auth_pop with "Dqst") as "Dqst"...
       iMod ("Commit" $! (circ_slice l t2 (b-1)) (SOMEV x) with "[◯]") as "HΦ".
-      { fr. rewrite -circ_slice_extend_right...
-        replace (S (b-1)) with b... }
-      iModIntro. iSplitL "Abst A Top Bot".
-      { iExists _,_,l. fr. fr. instantiate (1:=false)... }
+      { fr. rewrite -circ_slice_extend_right... replace (S (b-1)) with b... }
+      iModIntro. iSplitL "● Era Dqst C A T B".
+      { iExists _,_,l,t2. fr. fr. replace (Z.of_nat b - 1)%Z with (Z.of_nat (b - 1))%Z... }
       wp_pures.
 
       case_bool_decide... wp_pures.
-      rewrite rem_mod_eq...
+      replace (Z.of_nat b - 1)%Z with (Z.of_nat (b - 1))%Z... rewrite rem_mod_eq...
       wp_bind (! _)%E. iApply (wp_load_offset with "AOwn")...
       iIntros "!> AOwn". wp_pures.
       case_bool_decide... wp_pures.
-      iApply "HΦ". iExists _,_,_,_,_,l. fr.
+      iApply "HΦ". iExists _,_,_, _,l. fr.
     }
 
-    iModIntro. iSplitL "Abst A Top Bot".
-    { iExists _,_,l. fr. fr. instantiate (1:=true)... }
+    iModIntro. iSplitL "● Era Dqst C A T B".
+    { iExists _,_,l. fr. }
     wp_pures.
 
     case_bool_decide; wp_pures.
-    - (* empty *)
+    { (* empty *)
       assert (t2 = b)... subst t2.
       (* 3. roll back bot *)
       wp_bind (_ <- _)%E.
-        iInv "Inv" as (era3 ca3 l3 t3 b3) "Invs".
-          iDestruct "Invs" as "(>%Htb3 & >Abst & >A & >Top & >Bot)".
-        iDestruct "Abst" as "(Glob & Q & Era)".
-          iDestruct (ghost_var_agree with "eraOwn Era") as "%Eq".
-          injection Eq as [= <- <-].
-        iCombine "Glob Q Era" as "Abst".
-        iDestruct "A" as "[C↦ arr↦]".
-          iDestruct (mapsto_agree with "COwn C↦") as "%Hl1". injection Hl1 as [= <-].
-        iCombine "C↦ arr↦" as "A".
-        iDestruct "Bot" as (Pop3) "[bot↦ pop]".
-          iDestruct (ghost_var_agree with "pop popOwn") as "%". subst Pop3.
-          iMod (ghost_var_update_2 false with "pop popOwn") as "[pop popOwn]"...
-          iDestruct (mapsto_agree with "bot↦ bOwn") as "%Eq".
-          injection Eq as [= Eq]. assert (b = b3)... subst b3. clear Eq.
-          iCombine "bot↦ bOwn" as "bot↦". wp_store.
-          iDestruct "bot↦" as "[bot↦ bOwn]".
-        iCombine "bot↦ pop" as "Bot".
+        iInv "Inv" as (era3 ca3 l3 t3 b3 pop3) ">Invs".
+          iDestruct "Invs" as "(%Htb3 & ● & Era & Dqst & C & A & T & B)".
+        iDestruct (ghost_var_agree with "eraOwn Era") as "%Eq"; injection Eq as [= <- <- <- <- <-].
+        iMod (ghost_var_update_halves (era, arr, l, b, false)
+          with "eraOwn Era") as "[eraOwn Era]".
+        iCombine "bOwn B" as "B". wp_store.
+        iDestruct "B" as "[bOwn B]".
+        iMod "AU" as (l') "[Cont [_ Commit]]".
+      iMod ("Commit" $! l' NONEV with "[Cont]") as "HΦ"...
+      iModIntro. iSplitL "● Era Dqst C A T B".
+      { iExists _,_,l. fr. }
+      wp_pures. iApply "HΦ". iExists _,_,_, _,l. fr.
+    }
+    
+    (* non-empty *)
+    replace (Z.of_nat b - 1)%Z with (Z.of_nat (b - 1))%Z... rewrite rem_mod_eq...
+    wp_bind (! _)%E.
+    destruct (mod_get_is_Some l (b-1)) as [v Hv]...
+    iApply (wp_load_offset with "AOwn")...
+    iIntros "!> AOwn". wp_pures.
+    
+    (* we already did normal case *)
+    case_bool_decide... wp_pures.
+    
+    (* 3. CAS for one-element case *)
+    assert (b = S t2)... subst b.
+    wp_bind (CmpXchg _ _ _)%E.
+      iInv "Inv" as (era3 ca3 l3 t3 b3 pop3) ">Invs".
+        iDestruct "Invs" as "(%Htb3 & ● & Era & Dqst & C & A & T & B)".
+      iDestruct (ghost_var_agree with "eraOwn Era") as "%Eq"; injection Eq as [= <- <- <- <- <-].
+    destruct (decide (t2 = t3)).
+    + (* success *)
+      subst t3. wp_cmpxchg_suc.
+        replace (Z.of_nat t2 + 1)%Z with (Z.of_nat (S t2))...
       iMod "AU" as (l') "[Cont [_ Commit]]".
-        iMod ("Commit" $! l' NONEV with "[Cont]") as "HΦ"...
-      iModIntro. iSplitL "Abst A Top Bot".
-      { iExists _,_,l. fr. fr. instantiate (1:=false)... }
-      wp_pures. iApply "HΦ".
-      iExists _,_,_,_,_,l. fr.
-    - (* non-empty *)
-      rewrite rem_mod_eq...
-      wp_bind (! _)%E.
-      destruct (mod_get_is_Some l (b-1)) as [v Hv]...
-      iApply (wp_load_offset with "AOwn")...
-      iIntros "!> AOwn". wp_pures.
-      
-      (* we already did normal case *)
-      case_bool_decide... wp_pures.
-      
-      (* 3. CAS for one-element case *)
-      assert (b = S t2)... subst b.
-      wp_bind (CmpXchg _ _ _)%E.
-        iInv "Inv" as (era3 ca3 l3 t3 b3) "Invs".
-          iDestruct "Invs" as "(>%Htb3 & >Abst & >A & >Top & >Bot)".
-        iDestruct "Abst" as "(Glob & Q & Era)".
-          iDestruct (ghost_var_agree with "eraOwn Era") as "%Eq".
-          injection Eq as [= <- <-].
-        iCombine "Glob Q Era" as "Abst".
-        iDestruct "A" as "[C↦ arr↦]".
-          iDestruct (mapsto_agree with "COwn C↦") as "%Hl1". injection Hl1 as [= <-].
-        iCombine "C↦ arr↦" as "A".
-        iDestruct "Bot" as (Pop3) "[bot↦ pop]".
-          iDestruct (ghost_var_agree with "pop popOwn") as "%". subst Pop3.
-          iDestruct (mapsto_agree with "bot↦ bOwn") as "%Eq".
-          injection Eq as [= Eq]. assert (S t2 = b3)... subst b3. clear Eq.
-        iCombine "bot↦ pop" as "Bot".
-      destruct (decide (t2 = t3)).
-      + (* success *)
-        subst t3. wp_cmpxchg_suc.
-          replace (Z.of_nat t2 + 1)%Z with (Z.of_nat (S t2))...
-        iMod "AU" as (l') "[Cont [_ Commit]]".
-          iDestruct "Cont" as (γq' γpop' γera' γglob') "[%Enc' ◯]".
-            encode_agree Enc.
-          destruct (mod_get_is_Some l (S t2 - 1)) as [x Hx]...
-            rewrite Hv in Hx. injection Hx as [= <-].
-          iDestruct "Abst" as "(Glob & Q & Era)".
-            iMod (dqst_auth_update with "Glob") as "Glob"...
-            iDestruct (own_ea_agree with "Q ◯") as "%Eq". subst l'.
-            iMod (own_ea_update [] with "Q ◯") as "[Q ◯]".
-          iCombine "Glob Q Era" as "Abst".
-          iDestruct "Bot" as "[bot↦ pop]".
-            iMod (ghost_var_update_2 true with "pop popOwn") as "[pop popOwn]"...
-          iCombine "bot↦ pop" as "Bot".
-        iMod ("Commit" $! [] (SOMEV v) with "[◯]") as "HΦ".
-        { fr. rewrite (circ_slice_extend_right _ _ _ v)...
-          1: rewrite circ_slice_nil...
-          replace t2 with (S t2 - 1)... }
-        iModIntro. iSplitL "Abst A Top Bot".
-        { iExists era, arr, l, (S t2), (S t2).
-          rewrite circ_slice_nil... fr. iExists true... }
-        wp_pures.
+        iDestruct "Cont" as (γq' γera' γdqst') "[%Enc' ◯]". encode_agree Enc.
+        destruct (mod_get_is_Some l (S t2 - 1)) as [x Hx]...
+          rewrite Hv in Hx. injection Hx as [= <-].
+        iMod (dqst_auth_update with "Dqst") as "Dqst"...
+        iDestruct (own_ea_agree with "● ◯") as "%Eq". subst l'.
+        iMod (own_ea_update [] with "● ◯") as "[● ◯]".
+      iMod ("Commit" $! [] (SOMEV v) with "[◯]") as "HΦ".
+      { fr. rewrite (circ_slice_extend_right _ _ _ v)...
+        1: rewrite circ_slice_nil... replace t2 with (S t2 - 1)... }
+      iModIntro. iSplitL "● Era Dqst C A T B".
+      { iExists era, arr, l, (S t2), (S t2).
+        rewrite circ_slice_nil... fr. fr. }
+      wp_pures.
 
-        (* 4. roll back bot *)
-        wp_bind (_ <- _)%E.
-          iInv "Inv" as (era4 ca4 l4 t4 b4) "Invs".
-            iDestruct "Invs" as "(>%Htb4 & >Abst & >A & >Top & >Bot)".
-          iDestruct "Abst" as "(Glob & Q & Era)".
-            iDestruct (ghost_var_agree with "eraOwn Era") as "%Eq".
-            injection Eq as [= <- <-].
-          iCombine "Glob Q Era" as "Abst".
-          iDestruct "A" as "[C↦ arr↦]".
-            iDestruct (mapsto_agree with "COwn C↦") as "%Hl1". injection Hl1 as [= <-].
-          iCombine "C↦ arr↦" as "A".
-          iDestruct "Bot" as (Pop5) "[bot↦ pop]".
-            iDestruct (ghost_var_agree with "pop popOwn") as "%". subst Pop5.
-            iMod (ghost_var_update_2 false with "pop popOwn") as "[pop popOwn]"...
-            iDestruct (mapsto_agree with "bot↦ bOwn") as "%Eq".
-            injection Eq as [= Eq]. assert (S t2 = b4)... subst b4. clear Eq.
-            iCombine "bot↦ bOwn" as "bot↦". wp_store.
-              replace (Z.of_nat t2 + 1)%Z with (Z.of_nat (S t2))%Z...
-            iDestruct "bot↦" as "[bot↦ bOwn]".
-          iCombine "bot↦ pop" as "Bot".
-        iModIntro. iSplitL "Abst A Top Bot".
-        { iExists _,_,l. fr. fr. instantiate (1:=false)... }
-        wp_pures. iApply "HΦ".
-        iExists _,_,_,_,_,l. fr.
-      + (* fail *)
-        wp_cmpxchg_fail. { intro NO. injection NO... }
-        iMod "AU" as (l') "[Cont [_ Commit]]".
-        iMod ("Commit" $! l' NONEV with "[Cont]") as "HΦ"...
-        iModIntro. iSplitL "Abst A Top Bot".
-        { iExists _,_,l. fr. fr. instantiate (1:=true)... }
-        wp_pures.
+      (* 4. roll back bot *)
+      wp_bind (_ <- _)%E.
+        iInv "Inv" as (era4 ca4 l4 t4 b4 pop4) ">Invs".
+          iDestruct "Invs" as "(%Htb4 & ● & Era & Dqst & C & A & T & B)".
+        iDestruct (ghost_var_agree with "eraOwn Era") as "%Eq"; injection Eq as [= <- <- <- <- <-].
+        replace (Z.of_nat (S t2 - 1))%Z with (Z.of_nat t2)%Z...
+        replace (Z.of_nat (S t2) - 1)%Z with (Z.of_nat t2)%Z...
+        iMod (ghost_var_update_halves (era, arr, l, S t2, false)
+          with "eraOwn Era") as "[eraOwn Era]".
+        iCombine "bOwn B" as "B". wp_store.
+          replace (Z.of_nat t2 + 1)%Z with (Z.of_nat (S t2))%Z...
+        iDestruct "B" as "[bOwn B]".
+      iModIntro. iSplitL "● Era Dqst C A T B".
+      { iExists _,_,l. fr. }
+      wp_pures. iApply "HΦ". iExists _,_,_, _,l. fr.
+    + (* fail *)
+      wp_cmpxchg_fail. { intro NO. injection NO... }
+      iMod "AU" as (l') "[Cont [_ Commit]]".
+      iMod ("Commit" $! l' NONEV with "[Cont]") as "HΦ"...
+      iModIntro. iSplitL "● Era Dqst C A T B".
+      { iExists _,_,l. fr. }
+      wp_pures.
 
-        (* 4. roll back bot *)
-        wp_bind (_ <- _)%E.
-          iInv "Inv" as (era4 ca4 l4 t4 b4) "Invs".
-            iDestruct "Invs" as "(>%Htb4 & >Abst & >A & >Top & >Bot)".
-          iDestruct "Abst" as "(Glob & Q & Era)".
-            iDestruct (ghost_var_agree with "eraOwn Era") as "%Eq".
-            injection Eq as [= <- <-].
-          iCombine "Glob Q Era" as "Abst".
-          iDestruct "A" as "[C↦ arr↦]".
-            iDestruct (mapsto_agree with "COwn C↦") as "%Hl1". injection Hl1 as [= <-].
-          iCombine "C↦ arr↦" as "A".
-          iDestruct "Bot" as (Pop5) "[bot↦ pop]".
-            iDestruct (ghost_var_agree with "pop popOwn") as "%". subst Pop5.
-            iMod (ghost_var_update_2 false with "pop popOwn") as "[pop popOwn]"...
-            iDestruct (mapsto_agree with "bot↦ bOwn") as "%Eq".
-            injection Eq as [= Eq]. assert (S t2 = b4)... subst b4. clear Eq.
-            iCombine "bot↦ bOwn" as "bot↦". wp_store.
-              replace (Z.of_nat t2 + 1)%Z with (Z.of_nat (S t2))%Z...
-            iDestruct "bot↦" as "[bot↦ bOwn]".
-          iCombine "bot↦ pop" as "Bot".
-        iModIntro. iSplitL "Abst A Top Bot".
-        { iExists _,_,l. fr. fr. instantiate (1:=false)... }
-        wp_pures. iApply "HΦ".
-        iExists _,_,_,_,_,l. fr.
+      (* 4. roll back bot *)
+      wp_bind (_ <- _)%E.
+        iInv "Inv" as (era4 ca4 l4 t4 b4 pop4) ">Invs".
+          iDestruct "Invs" as "(%Htb4 & ● & Era & Dqst & C & A & T & B)".
+        iDestruct (ghost_var_agree with "eraOwn Era") as "%Eq"; injection Eq as [= <- <- <- <- <-].
+        replace (Z.of_nat (S t2 - 1))%Z with (Z.of_nat t2)%Z...
+        replace (Z.of_nat (S t2) - 1)%Z with (Z.of_nat t2)%Z...
+        iMod (ghost_var_update_halves (era, arr, l, S t2, false)
+          with "eraOwn Era") as "[eraOwn Era]".
+        iCombine "bOwn B" as "B". wp_store.
+          replace (Z.of_nat t2 + 1)%Z with (Z.of_nat (S t2))%Z...
+        iDestruct "B" as "[bOwn B]".
+      iModIntro. iSplitL "● Era Dqst C A T B".
+      { iExists _,_,l. fr. }
+      wp_pures. iApply "HΦ". iExists _,_,_, _,l. fr.
   Qed.
 
   Lemma steal_spec γ q :
@@ -1279,7 +1093,7 @@ Section proof.
       RET ov >>>.
   Proof with extended_auto.
     iIntros "#Is" (Φ) "AU".
-    iDestruct "Is" as (γq' γpop' γera' γglob') "Inv".
+    iDestruct "Is" as (γq' γera' γdqst') "Inv".
       iDestruct "Inv" as (C' top' bot') "Inv".
       iDestruct "Inv" as "(%Q & %Enc' & Inv)".
       subst q.
@@ -1288,40 +1102,40 @@ Section proof.
     (* 1. load top *)
     wp_bind (! _)%E.
       iInv "Inv" as (era1 ca1 l1 t1 b1) "Invs".
-        iDestruct "Invs" as "(>%Htb1 & >Abst & >A & >Top & >Bot)".
-      iDestruct "Abst" as "(Glob & Q & Era)".
-        iDestruct (dqst_get_frag with "Glob") as "#F1".
-      iCombine "Glob Q Era" as "Abst".
+        iDestruct "Invs" as "(%Htb1 & ● & Era & Dqst & C & A & T & B)".
+      iDestruct "Abst" as "(Dqst & Q & Era)".
+        iDestruct (dqst_get_frag with "Dqst") as "#F1".
+      iCombine "Dqst Q Era" as "Abst".
       wp_load.
-    iModIntro. iSplitL "Abst A Top Bot".
+    iModIntro. iSplitL "● Era Dqst C A T B".
     { iExists _,_,l1. fr. }
     wp_pures.
 
     (* 2. load bot *)
     wp_bind (! _)%E.
       iInv "Inv" as (era2 ca2 l2 t2 b2) "Invs".
-        iDestruct "Invs" as "(>%Htb2 & >Abst & >A & >Top & >Bot)".
-      iDestruct "Abst" as "(Glob & Q & Era)".
-        iDestruct (dqst_get_frag with "Glob") as "#F2".
-        iDestruct (dqst_get_lb with "Glob F1") as "%Lb12".
-      iCombine "Glob Q Era" as "Abst".
+        iDestruct "Invs" as "(%Htb2 & ● & Era & Dqst & C & A & T & B)".
+      iDestruct "Abst" as "(Dqst & Q & Era)".
+        iDestruct (dqst_get_frag with "Dqst") as "#F2".
+        iDestruct (dqst_get_lb with "Dqst F1") as "%Lb12".
+      iCombine "Dqst Q Era" as "Abst".
       iDestruct "Bot" as (Pop2) "[bot↦ Pop]". wp_load.
       iCombine "bot↦ Pop" as "Bot".
-    iModIntro. iSplitL "Abst A Top Bot".
+    iModIntro. iSplitL "● Era Dqst C A T B".
     { iExists _,_,l2. fr. }
     wp_pures.
 
     (* 3. load array *)
     wp_bind (! _)%E.
       iInv "Inv" as (era3 ca3 l3 t3 b3) "Invs".
-        iDestruct "Invs" as "(>%Htb3 & >Abst & >A & >Top & >Bot)".
-      iDestruct "Abst" as "(Glob & Q & Era)".
-        iDestruct (dqst_get_frag with "Glob") as "#F3".
-        iDestruct (dqst_get_lb with "Glob F2") as "%Lb23".
-      iCombine "Glob Q Era" as "Abst".
+        iDestruct "Invs" as "(%Htb3 & ● & Era & Dqst & C & A & T & B)".
+      iDestruct "Abst" as "(Dqst & Q & Era)".
+        iDestruct (dqst_get_frag with "Dqst") as "#F3".
+        iDestruct (dqst_get_lb with "Dqst F2") as "%Lb23".
+      iCombine "Dqst Q Era" as "Abst".
       iDestruct "A" as "[C↦ arr↦]". wp_load.
       iCombine "C↦ arr↦" as "A".
-    iModIntro. iSplitL "Abst A Top Bot".
+    iModIntro. iSplitL "● Era Dqst C A T B".
     { iExists _,_,l3. fr. }
     wp_pures.
 
@@ -1336,11 +1150,11 @@ Section proof.
     rewrite rem_mod_eq...
     wp_bind (! _)%E.
       iInv "Inv" as (era4 ca4 l4 t4 b4) "Invs".
-        iDestruct "Invs" as "(>%Htb4 & >Abst & >A & >Top & >Bot)".
-      iDestruct "Abst" as "(Glob & Q & Era)".
-        iDestruct (dqst_get_frag with "Glob") as "#F4".
-        iDestruct (dqst_get_lb with "Glob F3") as "%Lb34".
-      iCombine "Glob Q Era" as "Abst".
+        iDestruct "Invs" as "(%Htb4 & ● & Era & Dqst & C & A & T & B)".
+      iDestruct "Abst" as "(Dqst & Q & Era)".
+        iDestruct (dqst_get_frag with "Dqst") as "#F4".
+        iDestruct (dqst_get_lb with "Dqst F3") as "%Lb34".
+      iCombine "Dqst Q Era" as "Abst".
     destruct (decide (era3 = era4)) as [eqγ|neqγ].
     - (* array was not archived *)
       subst era4.
@@ -1351,24 +1165,24 @@ Section proof.
           iApply (wp_load_offset with "arr↦")...
           iIntros "!> arr↦".
         iCombine "C↦ arr↦" as "A".
-      iModIntro. iSplitL "Abst A Top Bot".
+      iModIntro. iSplitL "● Era Dqst C A T B".
       { iExists _,_,l4. fr. }
       wp_pures.
       
       (* 5. CAS *)
       wp_bind (CmpXchg _ _ _)%E.
       iInv "Inv" as (era5 ca5 l5 t5 b5) "Invs".
-        iDestruct "Invs" as "(>%Htb5 & >Abst & A & >Top & >Bot)".
-        iDestruct "Abst" as "(Glob & Q & Era)".
-          iDestruct (dqst_get_frag with "Glob") as "#F5".
-          iDestruct (dqst_get_lb with "Glob F4") as "%Lb45".
-        iCombine "Glob Q Era" as "Abst".
+        iDestruct "Invs" as "(%Htb5 & ● & Era & Dqst & C & A & T & B)".
+        iDestruct "Abst" as "(Dqst & Q & Era)".
+          iDestruct (dqst_get_frag with "Dqst") as "#F5".
+          iDestruct (dqst_get_lb with "Dqst F4") as "%Lb45".
+        iCombine "Dqst Q Era" as "Abst".
       destruct (decide (t1 = t5)); last first.
       { (* fail *)
         wp_cmpxchg_fail. { intro NO. inversion NO... }
         iMod "AU" as (lau) "[Cont [_ Commit]]".
         iMod ("Commit" $! lau NONEV with "[Cont]") as "HΦ"...
-        iModIntro. iSplitL "Abst A Top Bot".
+        iModIntro. iSplitL "● Era Dqst C A T B".
         { iExists _,_,l5. fr. }
         wp_pures. iApply "HΦ"...
       }
@@ -1383,52 +1197,52 @@ Section proof.
         { replace (mod_get l5 t1) with (mod_get l4 t1)...
           apply Lb45... }
       iMod "AU" as (lau) "[Cont [_ Commit]]".
-        iDestruct "Cont" as (γq'' γpop'' γera'' γglob'') "[%Enc'' ◯]".
+        iDestruct "Cont" as (γq'' γpop'' γera'' γdqst'') "[%Enc'' ◯]".
           encode_agree Enc'.
-        iDestruct "Abst" as "(Glob & Q & Era)".
+        iDestruct "Abst" as "(Dqst & Q & Era)".
           iDestruct (own_ea_agree with "Q ◯") as "%Hlau". subst lau.
           rewrite (circ_slice_shrink_left _ _ _ v)...
           iMod (own_ea_update (circ_slice l5 (S t1) b5)
             with "Q ◯") as "[Q ◯]".
-          iMod (dqst_auth_update with "Glob") as "Glob"...
-        iCombine "Glob Q Era" as "Abst".
+          iMod (dqst_auth_update with "Dqst") as "Dqst"...
+        iCombine "Dqst Q Era" as "Abst".
       iMod ("Commit" $! (circ_slice l5 (S t1) b5) (SOMEV v)
         with "[◯]") as "HΦ"; fr.
-      iModIntro. iSplitL "Abst A Top Bot".
+      iModIntro. iSplitL "● Era Dqst C A T B".
       { iExists _,_,l5. fr. fr. }
       wp_pures. iApply "HΦ"...
     - (* array was archived *)
-      iDestruct "Abst" as "(Glob & ● & Era)".
-        iDestruct (dqst_get_archived with "Glob F3")
+      iDestruct "Abst" as "(Dqst & ● & Era)".
+        iDestruct (dqst_get_archived with "Dqst F3")
           as (l' t' b') "#Arch"...
-      iCombine "Glob ● Era" as "Abst".
+      iCombine "Dqst ● Era" as "Abst".
       iDestruct (dqst_archived_get_lb with "Arch F3") as "%Ht3'".
         iDestruct (dqst_archived_get_frag with "Arch") as "F'".
-        iDestruct "Abst" as "(Glob & ● & Era)".
-          iDestruct (dqst_get_lb with "Glob F'") as "%Lb'4".
-        iCombine "Glob ● Era" as "Abst".
+        iDestruct "Abst" as "(Dqst & ● & Era)".
+          iDestruct (dqst_get_lb with "Dqst F'") as "%Lb'4".
+        iCombine "Dqst ● Era" as "Abst".
         iDestruct (dqst_frag_agree with "F3 F'") as "[_ %Hl3']".
         rewrite Hl3'. destruct (mod_get_is_Some l' t1) as [v Hv]...
         iDestruct (dqst_archived_get_array with "Arch") as "Parr".
       iApply (wp_persistent_load_offset with "Parr")...
-      iIntros "!> _ !>". iSplitL "Abst A Top Bot".
+      iIntros "!> _ !>". iSplitL "● Era Dqst C A T B".
       { iExists _,_,l4. fr. }
       wp_pures.
 
       (* 5. CAS *)
       wp_bind (CmpXchg _ _ _)%E.
       iInv "Inv" as (era5 ca5 l5 t5 b5) "Invs".
-        iDestruct "Invs" as "(>%Htb5 & >Abst & A & >Top & >Bot)".
-        iDestruct "Abst" as "(Glob & Q & Era)".
-          iDestruct (dqst_get_frag with "Glob") as "#F5".
-          iDestruct (dqst_get_lb with "Glob F4") as "%Lb45".
-        iCombine "Glob Q Era" as "Abst".
+        iDestruct "Invs" as "(%Htb5 & ● & Era & Dqst & C & A & T & B)".
+        iDestruct "Abst" as "(Dqst & Q & Era)".
+          iDestruct (dqst_get_frag with "Dqst") as "#F5".
+          iDestruct (dqst_get_lb with "Dqst F4") as "%Lb45".
+        iCombine "Dqst Q Era" as "Abst".
       destruct (decide (t1 = t5)); last first.
       { (* fail *)
         wp_cmpxchg_fail. { intro NO. inversion NO... }
         iMod "AU" as (lau) "[Cont [_ Commit]]".
         iMod ("Commit" $! lau NONEV with "[Cont]") as "HΦ"...
-        iModIntro. iSplitL "Abst A Top Bot".
+        iModIntro. iSplitL "● Era Dqst C A T B".
         { iExists _,_,l5. fr. }
         wp_pures. iApply "HΦ"...
       }
@@ -1445,18 +1259,18 @@ Section proof.
           - rewrite -Hv. symmetry. apply Lb'4...
           - apply Lb45... }
       iMod "AU" as (lau) "[Cont [_ Commit]]".
-        iDestruct "Cont" as (γq'' γpop'' γera'' γglob'') "[%Enc'' ◯]".
+        iDestruct "Cont" as (γq'' γpop'' γera'' γdqst'') "[%Enc'' ◯]".
           encode_agree Enc'.
-        iDestruct "Abst" as "(Glob & Q & Era)".
+        iDestruct "Abst" as "(Dqst & Q & Era)".
           iDestruct (own_ea_agree with "Q ◯") as "%Hlau". subst lau.
           rewrite (circ_slice_shrink_left _ _ _ v)...
           iMod (own_ea_update (circ_slice l5 (S t1) b5)
             with "Q ◯") as "[Q ◯]".
-          iMod (dqst_auth_update with "Glob") as "Glob"...
-        iCombine "Glob Q Era" as "Abst".
+          iMod (dqst_auth_update with "Dqst") as "Dqst"...
+        iCombine "Dqst Q Era" as "Abst".
       iMod ("Commit" $! (circ_slice l5 (S t1) b5) (SOMEV v)
         with "[◯]") as "HΦ"; fr.
-      iModIntro. iSplitL "Abst A Top Bot".
+      iModIntro. iSplitL "● Era Dqst C A T B".
       { iExists _,_,l5. fr. fr. }
       wp_pures. iApply "HΦ"...
   Qed.
